test/Mutable/thunk1.lean
@@ -12,27 +12,39 @@ protected def Thunk'.pure (a : α) : Thunk' α :=
   .mk fun _ ↦ a
 
 protected def Thunk'.get (x : Thunk' α) : α :=
-  Mutable.getWith₂ x (fun f ↦ f ()) (fun a _ ↦ a) (fun _ ↦ rfl)
+  Mutable.getModify₂ x (fun f ↦ let a := f (); ⟨a, fun _ ↦ a⟩) (fun _ ↦ rfl)
+
+@[inline] protected def Thunk'.map (f : α → β) (x : Thunk' α) : Thunk' β :=
+  .mk fun _ => f x.get
+
+@[inline] protected def Thunk'.bind (x : Thunk' α) (f : α → Thunk' β) : Thunk' β :=
+  .mk fun _ => (f x.get).get
 
 /-! lean4/tests/lean/thunk.lean -/
 
-#eval (Thunk.pure 1).get
-#eval (Thunk.mk fun _ => 2).get
+#eval (Thunk'.pure 1).get
+#eval (Thunk'.mk fun _ => 2).get
 #eval
-  let t1 := Thunk.mk fun _ => dbg_trace 4; 5
-  let t2 := Thunk.mk fun _ => dbg_trace 3; 0
-  let v2 := t2.get
+  let t1 := Thunk'.mk fun _ => dbg_trace 4; 5
+  -- let t2 := Thunk'.mk fun _ => dbg_trace 3; 0
+  -- let v2 := t2.get
+  let v2 := dbg_trace 3; 0
+
   let v1 := t1.get
   v1 + v2
 #eval
-  let t1 := Thunk.pure 8 |>.map fun n => dbg_trace 7; n
-  let t2 := Thunk.mk fun _ => dbg_trace 6; 0
-  let v2 := t2.get
+  let t1 := Thunk'.pure 8 |>.map fun n => dbg_trace 7; n
+  -- let t2 := Thunk'.mk fun _ => dbg_trace 6; 0
+  -- let v2 := t2.get
+  let v2 := dbg_trace 6; 0
+
   let v1 := t1.get
   v1 + v2
 #eval
-  let t1 := Thunk.pure 11 |>.bind fun n => dbg_trace 10; Thunk.pure n
-  let t2 := Thunk.mk fun _ => dbg_trace 9; 0
-  let v2 := t2.get
+  let t1 := Thunk'.pure 11 |>.bind fun n => dbg_trace 10; Thunk'.pure n
+  -- let t2 := Thunk'.mk fun _ => dbg_trace 9; 0
+  -- let v2 := t2.get
+  let v2 := dbg_trace 9; 0
+
   let v1 := t1.get
   v1 + v2
