test/Mutable/thunk2.lean
@@ -12,7 +12,7 @@ protected def Thunk'.pure (a : α) : Thunk' α :=
   .mk fun _ ↦ a
 
 protected def Thunk'.get (x : Thunk' α) : α :=
-  Mutable.getWith₂ x (fun f ↦ f ()) (fun a _ ↦ a) (fun _ ↦ rfl)
+  Mutable.getModify₂ x (fun f ↦ let a := f (); ⟨a, fun _ ↦ a⟩) (fun _ ↦ rfl)
 
 /-! lean4/tests/compiler/thunk.lean -/
 
@@ -23,8 +23,7 @@ def compute (v : Nat) : Thunk' Nat :=
 def test (t : Thunk' Nat) (n : Nat) : Nat :=
   n.repeat (fun r => t.get + r) 0
 
-def main : IO UInt32 :=
-  IO.println (toString (test (compute 1) 100000)) *>
-  pure 0
+def main : IO Unit :=
+  IO.println (toString (test (compute 1) 100000))
 
 #eval main
