Algorithm/Data/UnionFind.lean
@@ -1,0 +1,482 @@
+/-
+Copyright (c) 2024 Yuyang Zhao. All rights reserved.
+Released under Apache 2.0 license as described in the file LICENSE.
+Authors: Yuyang Zhao
+-/
+import Algorithm.Data.Classes.AssocArray
+import Algorithm.Data.MutableQuotient
+import Mathlib.Data.Set.Card
+
+namespace UnionFindImpl
+
+structure UnionFind (ι : Type*) [DecidableEq ι]
+    (P : Type*) [Inhabited P] [AssocDArray P ι ι id]
+    (S : Type*) [Inhabited S] [AssocArray S ι ℕ 1] where
+  parent : P
+  size : S
+  wf : WellFounded fun i j : ι ↦ i ≠ j ∧ i = parent[j]
+
+namespace UnionFind
+
+variable {ι : Type*} [DecidableEq ι]
+    {P : Type*} [Inhabited P] [AssocDArray P ι ι id]
+    {S : Type*} [Inhabited S] [AssocArray S ι ℕ 1]
+
+def rootCore (parent : P) (wf : WellFounded fun j k : ι ↦ j ≠ k ∧ j = parent[k]) (i : ι) : ι :=
+  let p := parent[i]
+  if p = i then
+    i
+  else
+    rootCore parent wf p
+termination_by WellFounded.wrap wf i
+decreasing_by simp_wf; tauto
+
+lemma rootCore_of_eq (parent : P) (wf : WellFounded fun j k : ι ↦ j ≠ k ∧ j = parent[k]) (i : ι)
+    (hi : parent[i] = i) : rootCore parent wf i = i := by
+  rw [rootCore, if_pos hi]
+
+@[simp]
+lemma rootCore_parent (parent : P) (wf : WellFounded fun j k : ι ↦ j ≠ k ∧ j = parent[k]) (i : ι) :
+    rootCore parent wf parent[i] = rootCore parent wf i := by
+  conv_rhs => rw [rootCore]
+  split_ifs with h
+  · rw [rootCore, h, if_pos h]
+  · rfl
+
+@[simp]
+lemma parent_rootCore (parent : P) (wf : WellFounded fun j k : ι ↦ j ≠ k ∧ j = parent[k]) (i : ι) :
+    parent[rootCore parent wf i] = rootCore parent wf i := by
+  rw [rootCore] -- TODO: use function induct in v4.8
+  split_ifs with h
+  · exact h
+  · exact parent_rootCore parent wf parent[i]
+termination_by WellFounded.wrap wf i
+decreasing_by simp_wf; tauto
+
+lemma transGen_rootCore (parent : P) (wf : WellFounded fun j k : ι ↦ j ≠ k ∧ j = parent[k])
+    (i : ι) (hi : parent[i] ≠ i) :
+    Relation.TransGen (fun i j ↦ i ≠ j ∧ i = parent[j]) (rootCore parent wf i) i := by
+  rw [rootCore, if_neg hi, rootCore] -- TODO: use function induct in v4.8
+  split_ifs with h
+  · exact .single ⟨hi, rfl⟩
+  · rw [rootCore_parent]
+    exact .tail (b := parent[i]) (transGen_rootCore parent wf parent[i] h) ⟨hi, rfl⟩
+termination_by WellFounded.wrap wf i
+decreasing_by simp_wf; tauto
+
+@[simp]
+lemma rootCore_eq_self (parent : P) (wf : WellFounded fun j k : ι ↦ j ≠ k ∧ j = parent[k])
+    (i : ι) : rootCore parent wf i = i ↔ parent[i] = i := by
+  constructor
+  · contrapose
+    exact fun hi ↦ @ne_of_irrefl _ _ wf.transGen.isIrrefl _ _ (transGen_rootCore parent wf i hi)
+  · exact rootCore_of_eq parent wf i
+
+def findAux (parent : P) (wf : WellFounded fun j k : ι ↦ j ≠ k ∧ j = parent[k]) (i : ι) :
+    ι × P :=
+  let p := parent[i]
+  if p = i then
+    ⟨i, parent⟩
+  else
+    let ⟨r, ps⟩ := findAux parent wf p
+    ⟨r, AssocDArray.set ps i r⟩
+termination_by WellFounded.wrap wf i
+decreasing_by simp_wf; tauto
+
+@[simp]
+lemma findAux_fst (parent : P) (wf : WellFounded fun j k : ι ↦ j ≠ k ∧ j = parent[k])
+    (i : ι) : (findAux parent wf i).fst = rootCore parent wf i := by
+  unfold findAux rootCore; dsimp -- TODO: use function induct in v4.8
+  split_ifs with hi
+  · rfl
+  · exact findAux_fst parent wf _
+termination_by WellFounded.wrap wf i
+decreasing_by simp_wf; tauto
+
+lemma findAux_snd_getElem (parent : P) (wf : WellFounded fun j k : ι ↦ j ≠ k ∧ j = parent[k])
+    (i j : ι) : (findAux parent wf i).snd[j] = parent[j] ∨
+      (findAux parent wf i).snd[j] = rootCore parent wf j := by
+  unfold findAux rootCore; dsimp -- TODO: use function induct in v4.8
+  split_ifs with hi
+  · exact .inl rfl
+  · obtain (hj | rfl) := decEq j i
+    · simp only [findAux_fst, AssocDArray.getElem_set, ne_eq, hj, not_false_eq_true,
+        Function.update_noteq, AssocDArray.get_eq_getElem]
+      exact (findAux_snd_getElem parent wf parent[i] j).imp_right (by rw [·, rootCore])
+    · simp [hi]
+termination_by WellFounded.wrap wf i
+decreasing_by simp_wf; tauto
+
+lemma wellFounded_findAux (parent : P) (wf : WellFounded fun j k : ι ↦ j ≠ k ∧ j = parent[k])
+    (i : ι) : WellFounded (fun j k : ι ↦ j ≠ k ∧ j = (findAux parent wf i).snd[k]) := by
+  refine Subrelation.wf (r := Relation.TransGen fun i j ↦ i ≠ j ∧ i = parent[j]) ?_ wf.transGen
+  rintro j k ⟨hj, rfl⟩
+  obtain (hk | hk) := findAux_snd_getElem parent wf i k
+  · exact .single ⟨hj, hk⟩
+  · rw [hk] at hj ⊢
+    exact transGen_rootCore parent wf k <| mt (rootCore_of_eq _ _ _) hj
+
+lemma rootCore_findAux_snd_apply (parent : P) (wf : WellFounded fun j k : ι ↦ j ≠ k ∧ j = parent[k])
+    (i : ι) (h) (j : ι) :
+    rootCore (findAux parent wf i).snd h j = rootCore parent wf j := by
+  unfold rootCore; dsimp -- TODO: use function induct in v4.8
+  obtain (H | H) := findAux_snd_getElem parent wf i j <;> rw [H]
+  · split_ifs with hj
+    · rfl
+    · exact rootCore_findAux_snd_apply parent wf i h parent[j]
+  · simp only [rootCore_eq_self, rootCore_parent]
+    split_ifs with hj
+    · rfl
+    · rw [rootCore_eq_self]
+      obtain (H | H) := findAux_snd_getElem parent wf i (rootCore parent wf j) <;> rw [H]
+      · exact parent_rootCore parent wf j
+      · rw [rootCore_eq_self, parent_rootCore]
+termination_by WellFounded.wrap wf j
+decreasing_by simp_wf; tauto
+
+@[simp]
+lemma rootCore_findAux_snd (parent : P) (wf : WellFounded fun j k : ι ↦ j ≠ k ∧ j = parent[k])
+    (i : ι) (h) :
+    rootCore (findAux parent wf i).snd h = rootCore parent wf := by
+  ext j; exact rootCore_findAux_snd_apply ..
+
+abbrev root (self : UnionFind ι P S) (i : ι) : ι :=
+  rootCore self.parent self.wf i
+
+lemma parent_root (self : UnionFind ι P S) (i : ι) :
+    self.parent[self.root i] = self.root i :=
+  parent_rootCore ..
+
+lemma root_eq_self (self : UnionFind ι P S) (i : ι) :
+    self.root i = i ↔ self.parent[i] = i :=
+  rootCore_eq_self self.parent self.wf i
+
+lemma root_of_parent_eq (self : UnionFind ι P S) (i : ι) (hi : self.parent[i] = i) :
+    self.root i = i :=
+  rootCore_of_eq self.parent self.wf i hi
+
+def find (self : UnionFind ι P S) (i : ι) :
+    ι × UnionFind ι P S :=
+  let ⟨parent, size, wf⟩ := self
+  match h : findAux parent wf i with
+  | ⟨r, ps⟩ => ⟨r, ⟨ps, size, (show _ = ps from congr_arg Prod.snd h) ▸ wellFounded_findAux _ _ _⟩⟩
+
+@[simp]
+lemma find_fst (self : UnionFind ι P S) (i : ι) :
+    (self.find i).fst = self.root i :=
+  findAux_fst self.parent self.wf i
+
+@[simp]
+lemma find_snd_root (self : UnionFind ι P S) (i : ι) :
+    (self.find i).snd.root = self.root :=
+  rootCore_findAux_snd self.parent self.wf i _
+
+lemma wellFounded_assocArraySet (parent : P) (wf : WellFounded fun j k : ι ↦ j ≠ k ∧ j = parent[k])
+    (i r : ι) (hr : parent[r] = r) :
+    WellFounded fun j k : ι ↦ j ≠ k ∧ j = (AssocArray.set parent i r)[k] := by
+  refine ⟨fun x ↦ ?_⟩
+  induction x using wf.induction with
+  | h x ih =>
+    refine ⟨x, fun p ⟨hpx, h⟩ ↦ ?_⟩
+    simp only [AssocDArray.getElem_set, Function.update, eq_rec_constant,
+      AssocDArray.get_eq_getElem, dite_eq_ite] at h
+    split_ifs at h with hx
+    · subst hx h
+      refine ⟨p, fun f hf ↦ ?_⟩
+      simp only [ne_eq, AssocDArray.getElem_set, Function.update, hpx, ↓reduceDite,
+        AssocDArray.get_eq_getElem, hr, not_and_self] at hf
+    · exact ih p ⟨hpx, h⟩
+
+set_option linter.unusedVariables false in -- easier to `rw` and `simp`
+@[inline, nolint unusedArguments]
+def setParent (parent : P) (size : S) (wf : WellFounded fun i j : ι ↦ i ≠ j ∧ i = parent[j])
+    (i j : ι) (hi : parent[i] = i) (hj : parent[j] = j) (s : ℕ) :
+    UnionFind ι P S :=
+  ⟨AssocDArray.set parent i j, AssocDArray.set size j s, wellFounded_assocArraySet parent wf i j hj⟩
+
+@[simp]
+lemma setParent_parent_eq_parent (parent : P) (size : S)
+    (wf : WellFounded fun i j : ι ↦ i ≠ j ∧ i = parent[j])
+    (i j : ι) (hi : parent[i] = i) (hj : parent[j] = j) (s : ℕ) (k : ι) :
+    (setParent parent size wf i j hi hj s).parent[k] = parent[k] ↔ k = i → j = parent[k] := by
+  simp [setParent, Function.update]
+
+@[simp]
+lemma setParent_parent_eq_self (parent : P) (size : S)
+    (wf : WellFounded fun i j : ι ↦ i ≠ j ∧ i = parent[j])
+    (i j : ι) (hi : parent[i] = i) (hj : parent[j] = j) (s : ℕ) (k : ι) :
+    (setParent parent size wf i j hi hj s).parent[k] = k ↔
+      (if k = i then j else parent[k]) = k := by
+  simp [setParent, Function.update]
+
+@[simp]
+lemma setParent_root (parent : P) (size : S) (wf : WellFounded fun i j : ι ↦ i ≠ j ∧ i = parent[j])
+    (i j : ι) (hi : parent[i] = i) (hj : parent[j] = j) (s : ℕ) (k : ι) :
+    (setParent parent size wf i j hi hj s).root k =
+      if rootCore parent wf k = i then j else rootCore parent wf k := by
+  unfold root rootCore; dsimp
+  obtain (hk | hk) := decEq parent[k] k <;> simp only [rootCore_parent, hk, ↓reduceIte]
+  · have hki : k ≠ i := by aesop
+    have : (setParent parent size wf i j hi hj s).parent[k] ≠ k := by
+      simp [ite_eq_iff, hki, hk]
+    simp only [this, ↓reduceIte]
+    convert setParent_root parent size wf i j hi hj s parent[k] using 1
+    · simp [← (setParent_parent_eq_parent parent size wf i j hi hj s k).mpr (absurd · hki)]
+    · simp
+  · simp only [setParent_parent_eq_self, setParent]
+    unfold rootCore
+    split_ifs <;> aesop
+termination_by WellFounded.wrap wf k
+decreasing_by simp_wf; tauto
+
+def link (self : UnionFind ι P S) (i j : ι) (hi : self.parent[i] = i) (hj : self.parent[j] = j) :
+    UnionFind ι P S :=
+  if i = j then
+    self
+  else
+    let ⟨parent, size, wf⟩ := self
+    let si := size[i]
+    let sj := size[j]
+    if si ≤ sj then
+      setParent parent size wf i j hi hj (si + sj)
+    else
+      setParent parent size wf j i hj hi (si + sj)
+
+@[simp]
+lemma link_root (self : UnionFind ι P S) (i j : ι) (hi : self.parent[i] = i)
+    (hj : self.parent[j] = j) :
+    (self.link i j hi hj).root = fun k ↦
+      if self.root k = i ∨ self.root k = j then
+        if self.size[i] ≤ self.size[j] then j else i
+      else
+        self.root k := by
+  -- ext k; unfold link; aesop -- slightly
+  ext k; unfold link; dsimp
+  obtain (hij | rfl) := decEq i j
+  · rw [if_neg hij]
+    split_ifs with hk hs <;> aesop
+  · aesop
+
+def union (self : UnionFind ι P S) (i j : ι) : UnionFind ι P S :=
+  match hi : self.find i with
+  | ⟨ri, uf₁⟩ =>
+    match hj : self.find j with
+    | ⟨rj, uf₂⟩ =>
+      link self ri rj
+        (by simp [← show _ = ri from congr_arg Prod.fst hi])
+        (by simp [← show _ = rj from congr_arg Prod.fst hj])
+
+@[simp]
+lemma union_root (self : UnionFind ι P S) (i j : ι) :
+    (self.union i j).root = fun k ↦
+      if self.root k = self.root i ∨ self.root k = self.root j then
+        if self.size[self.root i] ≤ self.size[self.root j] then self.root j else self.root i
+      else
+        self.root k := by
+  simp [union]
+
+instance : Inhabited (UnionFind ι P S) where
+  default := ⟨default, default, ⟨fun i ↦ ⟨i, by simp⟩⟩⟩
+
+@[simp]
+lemma default_parent : (default : UnionFind ι P S).parent = default :=
+  rfl
+
+@[simp]
+lemma default_size : (default : UnionFind ι P S).size = default :=
+  rfl
+
+@[simp]
+lemma default_root : (default : UnionFind ι P S).root = id := by
+  ext; simp
+
+def finsetOfRoot (self : UnionFind ι P S) (r : ι) : Finset ι :=
+  ((insert r (toDFinsupp' self.parent).support).filter (self.root · = r))
+
+lemma mem_finsetOfRoot_iff (self : UnionFind ι P S) (r i : ι) :
+    i ∈ self.finsetOfRoot r ↔ self.root i = r := by
+  simp? [finsetOfRoot] says
+    simp only [finsetOfRoot, id_eq, Finset.mem_filter, Finset.mem_insert,
+      DFinsupp'.mem_support_toFun, coe_toDFinsupp'_eq_get, AssocDArray.get_eq_getElem, ne_eq,
+      and_iff_right_iff_imp]
+  obtain (hr | hr) := decEq self.parent[i] i
+  · simp [hr]
+  · simp [hr, root, rootCore]
+
+instance (self : UnionFind ι P S) (r : ι) : Finite {i | self.root i = r} :=
+  Set.Finite.ofFinset (self.finsetOfRoot r) (self.mem_finsetOfRoot_iff r)
+
+def WF (self : UnionFind ι P S) : Prop :=
+  ∀ i : ι, self.parent[i] = i → self.size[i] = {j : ι | self.root j = i}.ncard
+
+lemma wf_congr {x y : UnionFind ι P S}
+    (hs : x.size = y.size) (hr : x.root = y.root) : x.WF ↔ y.WF := by
+  simp_rw [WF, ← root_eq_self, hs]; rw [hr]
+
+lemma wf_iff_size_root {self : UnionFind ι P S} :
+    self.WF ↔ ∀ i, self.size[self.root i] = {j : ι | self.root j = self.root i}.ncard :=
+  ⟨fun wf i ↦ wf (self.root i) (self.parent_root i),
+    fun h i hi ↦ self.root_of_parent_eq i hi ▸ h i⟩
+
+lemma default_wf : (default : UnionFind ι P S).WF :=
+  fun i ↦ by rw [default_root]; simp
+
+lemma setParent_wf (self : UnionFind ι P S)
+    (i j : ι) (hi : self.parent[i] = i) (hj : self.parent[j] = j) (hij : i ≠ j) (h : self.WF) :
+    (setParent self.parent self.size self.wf i j hi hj (self.size[i] + self.size[j])).WF := by
+  intro k hk
+  rw [setParent_parent_eq_self] at hk
+  conv_lhs =>
+    -- simp? [setParent, Function.update] says
+    simp only [setParent, AssocDArray.getElem_set, Function.update,
+      eq_rec_constant, AssocDArray.get_eq_getElem, dite_eq_ite]
+  split_ifs at hk ⊢ with hkj hki hki
+  · simp [← hki, ← hkj] at hij
+  · subst hkj
+    · conv_lhs => rw [h i hi, h k hk, ← Set.ncard_union_eq (by rw [Set.disjoint_iff]; intro; aesop)]
+      congr
+      ext x
+      simp? [setParent_root] says
+        simp only [Set.mem_union, Set.mem_setOf_eq, setParent_root,
+          ite_eq_left_iff]
+      rw [rootCore]
+      split_ifs with h
+      · rw [root_of_parent_eq _ _ h]; tauto
+      · rw [root, rootCore, if_neg h]; tauto
+  · simp [hk] at hkj
+  · rw [h k hk]
+    congr! 3
+    aesop
+
+lemma link_wf (self : UnionFind ι P S) (i j : ι) (hi : self.parent[i] = i) (hj : self.parent[j] = j)
+    (h : self.WF) : (self.link i j hi hj).WF := by
+  unfold link; dsimp
+  split_ifs with hij
+  · exact h
+  · exact setParent_wf _ _ _ _ _ hij h
+  · exact Nat.add_comm _ _ ▸ setParent_wf _ _ _ _ _ (Ne.symm hij) h
+
+lemma union_wf (self : UnionFind ι P S) (i j : ι) (h : self.WF) : (self.union i j).WF := by
+  unfold union; dsimp
+  exact self.link_wf _ _ _ _ h
+
+end UnionFind
+
+def UnionFindWF (ι : Type*) [DecidableEq ι]
+    (P : Type*) [Inhabited P] [AssocDArray P ι ι id]
+    (S : Type*) [Inhabited S] [AssocArray S ι ℕ 1] :=
+  { x : UnionFindImpl.UnionFind ι P S // x.WF }
+
+namespace UnionFindWF
+
+variable {ι : Type*} [DecidableEq ι]
+    {P : Type*} [Inhabited P] [AssocDArray P ι ι id]
+    {S : Type*} [Inhabited S] [AssocArray S ι ℕ 1]
+
+def IsRoot (self : UnionFindWF ι P S) (i : ι) : Prop := self.val.parent[i] = i
+
+abbrev root (self : UnionFindWF ι P S) (i : ι) : ι := self.val.root i
+
+lemma isRoot_iff_root {self : UnionFindWF ι P S} {i : ι} :
+    self.IsRoot i ↔ self.root i = i := by
+  simp [IsRoot]
+
+alias ⟨IsRoot.root_eq, _⟩ := isRoot_iff_root
+
+lemma IsRoot.root (self : UnionFindWF ι P S) (i : ι) :
+    self.IsRoot (self.root i) :=
+  isRoot_iff_root.mpr (by simp)
+
+abbrev find (self : UnionFindWF ι P S) (i : ι) :
+    ι × UnionFindWF ι P S :=
+  let ⟨x, hx⟩ := self
+  match h : x.find i with
+  | ⟨r, fx⟩ => ⟨r, ⟨fx, by
+    simpa only [← show _ = fx from congr_arg Prod.snd h,
+      UnionFind.wf_congr (by rfl) (x.find_snd_root i)]⟩⟩
+
+@[simp]
+lemma find_fst (self : UnionFindWF ι P S) (i : ι) :
+    (self.find i).fst = self.root i :=
+  self.val.find_fst i
+
+@[simp]
+lemma find_snd_root (self : UnionFindWF ι P S) (i : ι) :
+    (self.find i).snd.root = self.root :=
+  self.val.find_snd_root i
+
+abbrev union (self : UnionFindWF ι P S) (i j : ι) : UnionFindWF ι P S :=
+  ⟨self.val.union i j, self.val.union_wf i j self.prop⟩
+
+set_option linter.unusedVariables false in -- easier to `rw` and `simp`
+@[nolint unusedArguments]
+abbrev size (self : UnionFindWF ι P S) (i : ι) (hi : self.IsRoot i) : ℕ :=
+  self.val.size[i]
+
+lemma size_eq_of_root_eq (x y : UnionFindWF ι P S) (i : ι) (hxi : x.IsRoot i) (hyi : y.IsRoot i)
+    (h : x.root = y.root) : x.size i hxi = y.size i hyi := by
+  unfold root at h; simp [size, x.prop i hxi, y.prop i hyi, h]
+
+@[simp]
+lemma union_root (self : UnionFindWF ι P S) (i j : ι) :
+    (self.union i j).root = fun k ↦
+      if self.root k = self.root i ∨ self.root k = self.root j then
+        if self.size (self.root i) (.root _ _) ≤ self.size (self.root j) (.root _ _) then
+          self.root j
+        else
+          self.root i
+      else
+        self.root k :=
+  self.val.union_root i j
+
+end UnionFindWF
+
+end UnionFindImpl
+
+def UnionFind (ι : Type*) [DecidableEq ι]
+    (P : Type*) [Inhabited P] [AssocDArray P ι ι id]
+    (S : Type*) [Inhabited S] [AssocArray S ι ℕ 1] :=
+  MutableQuotient (UnionFindImpl.UnionFindWF ι P S) fun x ↦ x.root
+
+namespace UnionFind
+
+variable {ι : Type*} [DecidableEq ι]
+    {P : Type*} [Inhabited P] [AssocDArray P ι ι id]
+    {S : Type*} [Inhabited S] [AssocArray S ι ℕ 1]
+
+instance : Inhabited (UnionFind ι P S) where
+  default := .mk _ ⟨default, UnionFindImpl.UnionFind.default_wf⟩
+
+@[inline]
+def find (self : UnionFind ι P S) (i : ι) : ι :=
+  MutableQuotient.getModify self (fun x ↦ x.find i) (by simp (config := { contextual := true }))
+    (by simp)
+
+def IsRoot (self : UnionFind ι P S) (i : ι) : Prop := self.find i = i
+
+lemma find_isRoot (self : UnionFind ι P S) (i : ι) : self.IsRoot (self.find i) := by
+  induction self using MutableQuotient.ind
+  simp [IsRoot, find]
+
+@[inline]
+def union (self : UnionFind ι P S) (i j : ι) : UnionFind ι P S :=
+  MutableQuotient.map self (fun x ↦ x.union i j) fun _ _ h ↦ by
+    simp only [UnionFindImpl.UnionFindWF.union_root, h]
+    congr! 1
+    simp [h] -- `simp only [h]` made no progress
+    rw [UnionFindImpl.UnionFindWF.size_eq_of_root_eq (h := h)]
+    rw [UnionFindImpl.UnionFindWF.size_eq_of_root_eq (h := h)]
+
+@[inline]
+def size (self : UnionFind ι P S) (i : ι) (hi : self.IsRoot i) : ℕ :=
+  MutableQuotient.getMkEq self
+    (fun x hx ↦ x.size i (by
+      induction self using MutableQuotient.ind
+      rw [UnionFindImpl.UnionFindWF.isRoot_iff_root, hx, ← hi]
+      simp [find, getModify]))
+    (fun _ hx₁ _ hx₂ ↦ by
+      dsimp
+      rw [UnionFindImpl.UnionFindWF.size_eq_of_root_eq]
+      rw [hx₁, hx₂])
+
+end UnionFind
